Add automatic differentiation

theories/QcDual.v
@@ -1,4 +1,4 @@
-From Stdlib Require Import QArith Qcanon Ring.
+From Stdlib Require Import QArith Qcanon Ring Field.
 From DArith Require Import Dual.
 
 Module QcRing <: DRing.
@@ -53,3 +53,82 @@ Module QcRing <: DRing.
 End QcRing.
 
 Module QcDual := GDual QcRing.
+
+Module QcField <: DField.
+    Definition S := Qc.
+    Definition zero := 0%Qc.
+    Definition one := 1%Qc.
+    Definition add := Qcplus.
+    Definition mul := Qcmult.
+    Definition sub := Qcminus.
+    Definition opp := Qcopp.
+
+    Declare Scope S_scope.
+    Delimit Scope S_scope with S.
+    Notation "0" := zero : S_scope.
+    Notation "1" := one : S_scope.
+    Infix "+" := add (at level 50, left associativity) : S_scope.
+    Infix "-" := sub (at level 50, left associativity) : S_scope.
+    Infix "*" := mul (at level 40, left associativity) : S_scope.
+    Notation "- x" := (opp x) (at level 35, right associativity) : S_scope.
+
+    Definition eqb (x y : Qc) : bool :=
+        if Qc_eq_dec x y then true else false.
+
+    Lemma eqb_eq : forall s1 s2 : S, reflect (s1 = s2) (eqb s1 s2).
+    Proof.
+        intros. unfold eqb. destruct (Qc_eq_dec s1 s2).
+        - now apply ReflectT.
+        - now apply ReflectF.
+    Qed.
+
+    Lemma rt : ring_theory zero one add mul sub opp eq.
+    Proof. constructor; intros; unfold add,mul,sub,opp,zero,one; ring. Qed.
+
+    Lemma srt : semi_ring_theory zero one add mul eq.
+    Proof. constructor; intros; unfold add,mul,zero,one; ring. Qed.
+
+    Lemma zero_neq_one : (0 <> 1)%S.
+    Proof. unfold zero, one. discriminate. Qed.
+
+    Lemma opp_nonzero : forall x, (- x <> 0 <-> x <> 0)%S.
+    Proof.
+        intros x. unfold opp, zero. split; intro H; intro Hx.
+        - apply H. rewrite Hx. ring.
+        - apply H. rewrite <- (Qcopp_involutive x), Hx. ring.
+    Qed.
+
+    Lemma mul_nonzero : forall x y, (x <> 0 -> y <> 0 -> x * y <> 0)%S.
+    Proof.
+        intros x y Hx Hy. unfold mul, zero. intro H.
+        apply Qcmult_integral in H. destruct H; contradiction.
+    Qed.
+
+    (* Field-specific structure *)
+    Definition inv := Qcinv.
+    Definition div := Qcdiv.
+    Infix "/" := div (at level 40, left associativity) : S_scope.
+    Notation "/ x" := (inv x) (at level 35, right associativity) : S_scope.
+
+    Lemma div_def : forall x y, (x / y = x * inv y)%S.
+    Proof. intros. unfold div, inv, mul, Qcdiv. reflexivity. Qed.
+
+    Lemma mul_inv_r : forall x, (x <> 0)%S -> (x * inv x = 1)%S.
+    Proof.
+        intros x Hx. unfold mul, inv, one.
+        now apply Qcmult_inv_r.
+    Qed.
+
+    Lemma inv_0 : (inv 0 = 0)%S.
+    Proof. reflexivity. Qed.
+
+    Lemma ft : field_theory zero one add mul sub opp div inv eq.
+    Proof.
+        constructor.
+        - exact rt.
+        - unfold one, zero. discriminate.
+        - intros. unfold div, inv. reflexivity.
+        - intros p Hp. unfold mul, inv, one. apply Qcmult_inv_l.
+          unfold zero in Hp. exact Hp.
+    Qed.
+End QcField.
