examples/QcAD.v
@@ -1,0 +1,121 @@
+(* Automatic differentiation over the rationals *)
+
+From Stdlib Require Import QArith Qcanon Ring Field.
+From DArith Require Import Dual QcDual AD.
+
+Module QcAD := GDualAD QcField.
+Import QcAD Dual.
+
+Add Ring Qc_base_ring : QcField.rt.
+Add Field S_qc_field : QcField.ft.
+
+Open Scope Qc_scope.
+
+(* Test cases *)
+
+(* f(x) = x^2 *)
+Definition sq : Expr := Mul Var Var.
+
+(* f(x) = x^2 + 3x + 2 *)
+Definition poly : Expr :=
+    Add (Add (Mul Var Var) (Mul (Const (Q2Qc 3)) Var)) (Const (Q2Qc 2)).
+
+(* f(x) = 1 / x *)
+Definition recip : Expr := Div (Const 1) Var.
+
+(* f(x) = x / (x + 1) *)
+Definition frac : Expr := Div Var (Add Var (Const 1)).
+
+Lemma Q2Qc_2 : Q2Qc 2 = (1 + 1)%S.
+Proof. reflexivity. Qed.
+
+Lemma Q2Qc_3 : Q2Qc 3 = (1 + 1 + 1)%S.
+Proof. reflexivity. Qed.
+
+(* Symbolic derivatives *)
+
+(* d/dx x^2 = 2x. *)
+Example deriv_sq :
+    forall a, du (eval_dual sq ((a, 1%S : S) : D)) = (Q2Qc 2 * a)%S.
+Proof.
+    intro a.
+    assert (Hdef : defined_at sq a) by (cbn; tauto).
+    destruct (eval_dual_correct sq a Hdef) as [_ Hd].
+    change S with Qc in *. rewrite Hd, Q2Qc_2. cbn.
+    unfold one in *. ring.
+Qed.
+
+Add Field Qc_field : Qcft.
+
+(* d/dx (x^2 + 3x + 2) = 2x + 3. *)
+Example deriv_poly :
+    forall a, du (eval_dual poly (a, 1%S : S)) = (Q2Qc 2 * a + Q2Qc 3)%S.
+Proof.
+    intro a.
+    assert (Hdef : defined_at poly a) by (cbn; tauto).
+    destruct (eval_dual_correct poly a Hdef) as [_ Hd].
+    rewrite Hd. cbn.
+    rewrite Q2Qc_2, Q2Qc_3.
+    change S with Qc in *.
+    change QcField.add with Qcplus. change QcField.mul with Qcmult.
+    unfold zero, one. rewrite Qcmult_0_l, Qcplus_0_l, Qcplus_0_r.
+    ring.
+Qed.
+
+(* d/dx (1/x) = -1/x^2, where x <> 0. *)
+Example deriv_recip :
+    forall a, (a <> 0)%S ->
+        du (eval_dual recip (a, 1%S)) = (- Qcinv (a * a))%S.
+Proof.
+    intros a Ha.
+    assert (Hdef : defined_at recip a) by (cbn; tauto).
+    destruct (eval_dual_correct recip a Hdef) as [_ Hd].
+    change S with Qc in *. rewrite Hd. cbn.
+    unfold one, zero in *.
+    change QcField.add with Qcplus. change QcField.mul with Qcmult.
+    change QcField.sub with Qcminus. change QcField.opp with Qcopp.
+    unfold div.
+    now field.
+Qed.
+
+(* d/dx (x/(x+1)) = 1/(x+1)^2, where x + 1 <> 0. *)
+Example deriv_frac :
+    forall a, ((a + 1) <> 0)%S ->
+        du (eval_dual frac (a, 1%S)) = Qcinv ((a + 1) * (a + 1)).
+Proof.
+    intros a Ha.
+    assert (Hdef : defined_at frac a) by (cbn; tauto).
+    destruct (eval_dual_correct frac a Hdef) as [_ Hd].
+    change S with Qc in *. rewrite Hd. cbn.
+    unfold one, zero in *.
+    change QcField.add with Qcplus. change QcField.mul with Qcmult.
+    change QcField.sub with Qcminus. change QcField.opp with Qcopp.
+    unfold div. now field.
+Qed.
+
+(* f(x) = x^2 + 3x + 2 at x = 5:  value 42, derivative 13. *)
+Example poly_at_5_value :
+    real (eval_dual poly (Q2Qc 5, 1%S)) = Q2Qc 42.
+Proof. reflexivity. Qed.
+
+Example poly_at_5_deriv :
+    du (eval_dual poly (Q2Qc 5, 1%S)) = Q2Qc 13.
+Proof. reflexivity. Qed.
+
+(* f(x) = 1/x at x = 2:  value 1/2, derivative -1/4. *)
+Example recip_at_2_value :
+    real (eval_dual recip (Q2Qc 2, 1%S)) = Q2Qc (1 # 2).
+Proof. reflexivity. Qed.
+
+Example recip_at_2_deriv :
+    du (eval_dual recip (Q2Qc 2, 1%S)) = Q2Qc (- (1 # 4)).
+Proof. reflexivity. Qed.
+
+(* f(x) = x/(x+1) at x = 3:  value 3/4, derivative 1/16. *)
+Example frac_at_3_value :
+    real (eval_dual frac (Q2Qc 3, 1%S)) = Q2Qc (3 # 4).
+Proof. reflexivity. Qed.
+
+Example frac_at_3_deriv :
+    du (eval_dual frac (Q2Qc 3, 1%S)) = Q2Qc (1 # 16).
+Proof. apply Qceq_alt. reflexivity. Qed.
